examples/pseudo_bool/graph_encoding/subgraph_isoScript.sml
@@ -470,30 +470,12 @@ Proof
   metis_tac[encode_correct,PAIR,pbc_ge_thm]
 QED
 
-(* The normalised encoding *)
-Definition norm_encode_def:
-  norm_encode gp gt =
-  full_normalise (full_encode gp gt)
-End
-
 Theorem pbf_vars_full_encode:
   pbf_vars (set (full_encode gp gt)) ⊆ goodString
 Proof
   rw[SUBSET_DEF,full_encode_def,LIST_TO_SET_MAP,pbf_vars_IMAGE]>>
   simp[IN_DEF]>>
   metis_tac[enc_string_goodString,PAIR]
-QED
-
-Theorem norm_encode_correct:
-  good_graph gp ∧
-  good_graph gt ∧
-  norm_encode gp gt = constraints ⇒
-  (has_subgraph_iso gp gt ⇔ satisfiable (set constraints))
-Proof
-  rw[norm_encode_def]>>
-  DEP_REWRITE_TAC[full_normalise_satisfiable]>>rw[]
-  >- metis_tac[pbf_vars_full_encode]
-  >- metis_tac[full_encode_correct]
 QED
 
 (*
